cfrontend/Cexec.v
@@ -890,6 +890,7 @@ Fixpoint step_expr (cp: compartment) (k: kind) (a: expr) (m: mem): reducts expr 
           match classify_fun tyf with
           | fun_case_f tyargs tyres cconv =>
               do fd <- Genv.find_funct ge vf;
+              check (Policy.allowed_call_b pol cp fd);
               do vargs <- sem_cast_arguments vtl tyargs m;
               check type_eq (type_of_fundef fd) (Tfunction tyargs tyres cconv);
               topred (Callred "red_call" fd vargs ty m)
@@ -938,12 +939,12 @@ Inductive imm_safe_t (cp: compartment): kind -> expr -> mem -> Prop :=
       context RV to C ->
       imm_safe_t cp to (C r) m
   | imm_safe_t_callred: forall to C r m fd args ty,
-      callred ge r m fd args ty ->
+      callred pol ge cp r m fd args ty ->
       context RV to C ->
       imm_safe_t cp to (C r) m.
 
 Remark imm_safe_t_imm_safe:
-  forall cp k a m, imm_safe_t cp k a m -> imm_safe ge e cp k a m.
+  forall cp k a m, imm_safe_t cp k a m -> imm_safe pol ge e cp k a m.
 Proof.
   induction 1.
   constructor.
@@ -951,6 +952,7 @@ Proof.
   eapply imm_safe_lred; eauto.
   eapply imm_safe_rred; eauto.
   eapply imm_safe_callred; eauto.
+  inversion H; auto.
 Qed.
 
 Fixpoint exprlist_all_values (rl: exprlist) : Prop :=
@@ -1011,6 +1013,7 @@ Definition invert_expr_prop (cp: compartment) (a: expr) (m: mem) : Prop :=
       /\ Genv.find_funct ge vf = Some fd
       /\ cast_arguments m rargs tyargs vl
       /\ type_of_fundef fd = Tfunction tyargs tyres cconv
+      /\ Policy.allowed_call pol cp fd
   | Ebuiltin ef tyargs rargs ty =>
       exprlist_all_values rargs ->
       exists vargs t vres m' w',
@@ -1051,7 +1054,7 @@ Qed.
 
 Lemma callred_invert:
   forall cp r fd args ty m,
-  callred ge r m fd args ty ->
+  callred pol ge cp r m fd args ty ->
   invert_expr_prop cp r m.
 Proof.
   intros. inv H. simpl.
@@ -1147,7 +1150,7 @@ Definition reduction_ok (cp: compartment) (k: kind) (a: expr) (m: mem) (rd: redu
   match k, rd with
   | LV, Lred _ l' m' => lred ge e a m l' m'
   | RV, Rred _ r' m' t => rred ge cp a m t r' m' /\ exists w', possible_trace w t w'
-  | RV, Callred _ fd args tyres m' => callred ge a m fd args tyres /\ m' = m
+  | RV, Callred _ fd args tyres m' => callred pol ge cp a m fd args tyres /\ m' = m
   | LV, Stuckred => ~imm_safe_t cp k a m
   | RV, Stuckred => ~imm_safe_t cp k a m
   | _, _ => False
@@ -1501,13 +1504,18 @@ Proof with (try (apply not_invert_ok; simpl; intro; myinv; intuition congruence;
   (* top *)
   destruct (classify_fun tyf) as [tyargs tyres cconv|] eqn:?...
   destruct (Genv.find_funct ge vf) as [fd|] eqn:?...
+  destruct (Policy.allowed_call_b pol cp fd) eqn:?...
   destruct (sem_cast_arguments vtl tyargs m) as [vargs|] eqn:?...
   destruct (type_eq (type_of_fundef fd) (Tfunction tyargs tyres cconv))...
   apply topred_ok; auto. red. split; auto. eapply red_call; eauto.
   eapply sem_cast_arguments_sound; eauto.
+  eapply Policy.allowed_call_reflect; eauto.
   apply not_invert_ok; simpl; intros; myinv. specialize (H ALLVAL). myinv. congruence.
   apply not_invert_ok; simpl; intros; myinv. specialize (H ALLVAL). myinv.
   exploit sem_cast_arguments_complete; eauto. intros [vtl' [P Q]]. congruence.
+  apply not_invert_ok; simpl; intros; myinv. specialize (H ALLVAL). myinv.
+  match goal with H: Policy.allowed_call _ _ _ |- _ => apply Policy.allowed_call_reflect in H end.
+  congruence.
   apply not_invert_ok; simpl; intros; myinv. specialize (H ALLVAL). myinv. congruence.
   apply not_invert_ok; simpl; intros; myinv. specialize (H ALLVAL). myinv. congruence.
   (* depth *)
@@ -1630,12 +1638,14 @@ Qed.
 
 Lemma callred_topred:
   forall cp a fd args ty m,
-  callred ge a m fd args ty ->
+  callred pol ge cp a m fd args ty ->
   exists rule, step_expr cp RV a m = topred (Callred rule fd args ty m).
 Proof.
   induction 1; simpl.
   rewrite H2. exploit sem_cast_arguments_complete; eauto. intros [vtl [A B]].
-  rewrite A; rewrite H; rewrite B; rewrite H1; rewrite dec_eq_true. econstructor; eauto.
+  rewrite A; rewrite H; rewrite B; rewrite H1; rewrite dec_eq_true.
+  apply Policy.allowed_call_reflect in ALLOWED. rewrite ALLOWED.
+  econstructor; eauto.
 Qed.
 
 Definition reducts_incl {A B: Type} (C: A -> B) (res1: reducts A) (res2: reducts B) : Prop :=
@@ -1843,7 +1853,7 @@ Qed.
 
 Lemma imm_safe_imm_safe_t:
   forall cp k a m,
-  imm_safe ge e cp k a m ->
+  imm_safe pol ge e cp k a m ->
   imm_safe_t cp k a m \/
   exists C, exists a1, exists t, exists a1', exists m',
     context RV k C /\ a = C a1 /\ rred ge cp a1 m t a1' m' /\ forall w', ~possible_trace w t w'.
@@ -1870,7 +1880,7 @@ Theorem not_imm_safe_t:
   ~imm_safe_t f.(fn_comp) K a m ->
   Csem.step pol ge (ExprState f (C a) k e m) E0 Stuckstate \/ can_crash_world w (ExprState f (C a) k e m).
 Proof.
-  intros. destruct (classic (imm_safe ge e f.(fn_comp) K a m)).
+  intros. destruct (classic (imm_safe pol ge e f.(fn_comp) K a m)).
   exploit imm_safe_imm_safe_t; eauto.
   intros [A | [C1 [a1 [t [a1' [m' [A [B [D E]]]]]]]]]. contradiction.
   right. red. exists t; econstructor; split; auto.
@@ -2062,7 +2072,6 @@ Definition do_step (w: world) (s: state) : list transition :=
       end
 
   | Callstate (Internal f) vargs k m =>
-      check (Policy.allowed_call_b pol (call_comp k) f);
       check (list_norepet_dec ident_eq (var_names (fn_params f) ++ var_names (fn_vars f)));
       let (e,m1) := do_alloc_variables empty_env m (f.(fn_params) ++ f.(fn_vars)) in
       do m2 <- sem_bind_parameters w e m1 f.(fn_params) vargs;
@@ -2141,7 +2150,6 @@ Proof with try (left; right; econstructor; eauto; fail).
   myinv. left; right; apply step_internal_function with m1. auto.
   change e with (fst (e,m1)). change m1 with (snd (e,m1)) at 2. rewrite <- Heqp.
   apply do_alloc_variables_sound. eapply sem_bind_parameters_sound; eauto.
-  apply Policy.allowed_call_reflect; auto.
   (* external *)
   destruct p as [[[w' tr] v] m']. myinv. left; right; constructor.
   eapply do_ef_external_sound; eauto.
@@ -2152,7 +2160,7 @@ Proof with try (left; right; econstructor; eauto; fail).
 Qed.
 
 Remark estep_not_val:
-  forall f a k e m t S, estep ge (ExprState f a k e m) t S -> is_val a = None.
+  forall f a k e m t S, estep pol ge (ExprState f a k e m) t S -> is_val a = None.
 Proof.
   intros.
   assert (forall b from to C, context from to C -> (from = to /\ C = fun x => x) \/ is_val (C b) = None).
@@ -2193,7 +2201,8 @@ Proof with (unfold ret; eauto with coqlib).
   apply extensionality; auto.
 (* callred *)
   unfold do_step; rewrite NOTVAL.
-  exploit callred_topred; eauto. instantiate (1 := f.(fn_comp)). instantiate (1 := w). instantiate (1 := e).
+  exploit callred_topred; eauto.
+  instantiate (1 := w). instantiate (1 := e).
   intros (rule & STEP). exists rule.
   change (TR rule E0 (Callstate fd vargs (Kcall f e C ty k) m)) with (expr_final_state f k e (C, Callred rule fd vargs ty m)).
   apply in_map.
@@ -2232,7 +2241,6 @@ Proof with (unfold ret; eauto with coqlib).
   (* Call step *)
   rewrite pred_dec_true; auto. rewrite (do_alloc_variables_complete _ _ _ _ _ H1).
   rewrite (sem_bind_parameters_complete _ _ _ _ _ _ H2)...
-  rewrite ((proj1 (Policy.allowed_call_reflect _ _ _)) ALLOWED)...
   exploit do_ef_external_complete; eauto. intro EQ; rewrite EQ. auto with coqlib.
 Qed.
 
